Move ChainStep and ChainTrace to Type
This moves ChainStep and ChainTrace to type. The reason being that our
proofs will depend on prefixes of traces and it will be very useful (if
not required) to be able to match on the trace and the steps.
ChainBuilderType is changed appropriately: now, an implementation just
needs to prove that ChainTrace empty_env [] cur_env [] is inhabited.
Thus, ChainTrace can basically be seen as one particular way to order
the execution so that we reach a state. When it is inhabited, it thus
means that there exists a proper way to order actions so that we reach
the state we are in.

src/Blockchain.v
@@ -505,25 +505,23 @@ changes an environment and which external actions to execute after it. *)
 (* todo: handle deploy/call failures. We should still transfer gas and allow this
 to be recorded. *)
 Inductive ChainStep :
-  Environment -> Action -> Tx ->
-  Environment -> list Action -> Prop :=
+  Environment -> Action ->
+  Environment -> list Action -> Type :=
   | step_empty :
       forall {pre : Environment}
              {act : Action}
-             {tx : Tx}
              {new_env : Environment}
              (from to : Address)
              (amount : Amount),
         amount <= account_balance pre from ->
         address_is_contract to = false ->
         act = build_act from (act_transfer to amount) ->
-        tx = build_tx from to amount tx_empty ->
+        let tx := build_tx from to amount tx_empty in
         EnvironmentEquiv new_env (add_tx tx pre) ->
-        ChainStep pre act tx new_env []
+        ChainStep pre act new_env []
   | step_deploy :
       forall {pre : Environment}
              {act : Action}
-             {tx : Tx}
              {new_env : Environment}
              (from to : Address)
              (amount : Amount)
@@ -535,7 +533,9 @@ Inductive ChainStep :
       incoming_txs pre to = [] ->
       address_is_contract to = true ->
       act = build_act from (act_deploy amount wc setup) ->
-      tx = build_tx from to amount (tx_deploy (build_contract_deployment (wc_version wc) setup)) ->
+      let tx := build_tx
+                  from to amount
+                  (tx_deploy (build_contract_deployment (wc_version wc) setup)) in
       wc_init
         wc
         (add_tx tx pre)
@@ -544,11 +544,10 @@ Inductive ChainStep :
       EnvironmentEquiv
         new_env
         (set_contract_state to state (add_contract to wc (add_tx tx pre))) ->
-      ChainStep pre act tx new_env []
+      ChainStep pre act new_env []
   | step_call_empty :
       forall {pre : Environment}
              {act : Action}
-             {tx : Tx}
              {new_env : Environment}
              {new_acts : list Action}
              (from to : Address)
@@ -561,7 +560,7 @@ Inductive ChainStep :
       env_contracts pre to = Some wc ->
       contract_state pre to = Some prev_state ->
       act = build_act from (act_transfer to amount) ->
-      tx = build_tx from to amount tx_empty ->
+      let tx := build_tx from to amount tx_empty in
       wc_receive
         wc
         (add_tx tx pre)
@@ -572,11 +571,10 @@ Inductive ChainStep :
       EnvironmentEquiv
         new_env
         (set_contract_state to new_state (add_tx tx pre)) ->
-      ChainStep pre act tx new_env new_acts
+      ChainStep pre act new_env new_acts
   | step_call_msg :
       forall {pre : Environment}
              {act : Action}
-             {tx : Tx}
              {new_env : Environment}
              {new_acts : list Action}
              (from to : Address)
@@ -590,7 +588,7 @@ Inductive ChainStep :
       env_contracts pre to = Some wc ->
       contract_state pre to = Some prev_state ->
       act = build_act from (act_call to amount msg) ->
-      tx = build_tx from to amount (tx_call msg) ->
+      let tx := build_tx from to amount (tx_call msg) in
       wc_receive
         wc
         (add_tx tx pre)
@@ -601,49 +599,78 @@ Inductive ChainStep :
       EnvironmentEquiv
         new_env
         (set_contract_state to new_state (add_tx tx pre)) ->
-      ChainStep pre act tx new_env new_acts.
+      ChainStep pre act new_env new_acts.
+
+Section Accessors.
+Context {pre : Environment} {act : Action}
+        {post : Environment} {new_acts : list Action}
+        (step : ChainStep pre act post new_acts).
+
+Definition step_from : Address :=
+  match step with
+  | step_empty from _ _ _ _ _ _ _
+  | step_deploy from _ _ _ _ _ _ _ _ _ _ _ _ _
+  | step_call_empty from _ _ _ _ _ _ _ _ _ _ _ _ _ _
+  | step_call_msg from _ _ _ _ _ _ _ _ _ _ _ _ _ _ _ => from
+  end.
+
+Definition step_to : Address :=
+  match step with
+  | step_empty _ to _ _ _ _ _ _
+  | step_deploy _ to _ _ _ _ _ _ _ _ _ _ _ _
+  | step_call_empty _ to _ _ _ _ _ _ _ _ _ _ _ _ _
+  | step_call_msg _ to _ _ _ _ _ _ _ _ _ _ _ _ _ _ => to
+  end.
+
+Definition step_amount : Amount :=
+  match step with
+  | step_empty _ _ amount _ _ _ _ _
+  | step_deploy _ _ amount _ _ _ _ _ _ _ _ _ _ _
+  | step_call_empty _ _ amount _ _ _ _ _ _ _ _ _ _ _ _
+  | step_call_msg _ _ amount _ _ _ _ _ _ _ _ _ _ _ _ _ => amount
+  end.
+End Accessors.
 
 Section Theories.
-Section Single.
-Context {pre : Environment} {act : Action} {tx : Tx}
+Context {pre : Environment} {act : Action}
         {post : Environment} {new_acts : list Action}
-        (step : ChainStep pre act tx post new_acts).
+        (step : ChainStep pre act post new_acts).
 
 Lemma account_balance_post (addr : Address) :
-  (account_balance post addr =
+  account_balance post addr =
   account_balance pre addr
-  + (if (addr =? tx_to tx)%address then tx_amount tx else 0)
-  - (if (addr =? tx_from tx)%address then tx_amount tx else 0)).
+  + (if (addr =? step_to step)%address then step_amount step else 0)
+  - (if (addr =? step_from step)%address then step_amount step else 0).
 Proof.
   unfold account_balance.
-  destruct step;
+  destruct step; subst; cbn;
     match goal with
     | [H: EnvironmentEquiv _ _ |- _] => rewrite H
     end;
-    simpl; unfold add_tx_to_map; destruct_address_eq; simpl; lia.
+    cbn; unfold add_tx_to_map; destruct_address_eq; cbn; lia.
 Qed.
 
 Lemma account_balance_post_to :
-  tx_from tx <> tx_to tx ->
-  account_balance post (tx_to tx) =
-  account_balance pre (tx_to tx) + tx_amount tx.
+  step_from step <> step_to step ->
+  account_balance post (step_to step) =
+  account_balance pre (step_to step) + step_amount step.
 Proof.
   rewrite account_balance_post.
   destruct_address_eq; prove.
 Qed.
 
 Lemma account_balance_post_from :
-  tx_from tx <> tx_to tx ->
-  account_balance post (tx_from tx) =
-  account_balance pre (tx_from tx) - tx_amount tx.
+  step_from step <> step_to step ->
+  account_balance post (step_from step) =
+  account_balance pre (step_from step) - step_amount step.
 Proof.
   rewrite account_balance_post.
   destruct_address_eq; prove.
 Qed.
 
 Lemma account_balance_post_irrelevant (addr : Address) :
-  addr <> tx_from tx ->
-  addr <> tx_to tx ->
+  addr <> step_from step ->
+  addr <> step_to step ->
   account_balance post addr = account_balance pre addr.
 Proof.
   rewrite account_balance_post.
@@ -657,7 +684,6 @@ Proof.
     | [H: EnvironmentEquiv _ _ |- _] => now rewrite H
     end.
 Qed.
-End Single.
 End Theories.
 End Step.
 
@@ -701,10 +727,9 @@ Definition empty_env : Environment :=
 (* The ChainTrace captures that there is a valid execution where,
 starting from one environment and queue of actions, we end up in a
 different environment and queue of actions. *)
-Unset Elimination Schemes.
 Inductive ChainTrace :
   Environment -> list Action ->
-  Environment -> list Action -> Prop :=
+  Environment -> list Action -> Type :=
   | ctrace_refl :
       forall {env l}, ChainTrace env l env l
   (* Add a new block to the trace *)
@@ -730,11 +755,10 @@ Inductive ChainTrace :
              {prev_to : Environment}
              {act : Action}
              {acts : list Action}
-             {tx : Tx}
              {new : Environment}
              {new_acts : list Action},
         ChainTrace from from_queue prev_to (act :: acts) ->
-        ChainStep prev_to act tx new new_acts ->
+        ChainStep prev_to act new new_acts ->
         ChainTrace from from_queue new (new_acts ++ acts)
   (* Reorder action order *)
   | ctrace_permute :
@@ -745,17 +769,6 @@ Inductive ChainTrace :
         ChainTrace from from_queue to to_queue ->
         Permutation to_queue to_queue' ->
         ChainTrace from from_queue to to_queue'.
-
-(* The normal induction principle generated for propositions does not
-allow the picked proposition to depend on the inhabitant of the
-proposition. However, for our traces, we will often want to prove
-properties that rely on the specific inhabitant. For instance when we
-need to reason about prefixes or suffixes. Thus we derive a normal
-principle instead. As an example, rhis is necessary for the proofs
-about trace_app below. This difference between inductives in Prop and
-Type, and the solution was highlighted to me by Danil Annenkov. *)
-Scheme ChainTrace_ind := Induction for ChainTrace Sort Prop.
-Set Elimination Schemes.
 
 Fixpoint trace_app
             {from mid to : Environment}
@@ -822,7 +835,7 @@ Ltac rewrite_environment_equiv :=
 
 Ltac destruct_step :=
   match goal with
-  | [H: ChainStep _ _ _ _ _ |- _] => destruct H
+  | [H: ChainStep _ _ _ _ |- _] => destruct H
   end.
 
 Lemma contract_addr_format
@@ -862,7 +875,7 @@ Class ChainBuilderType :=
       option builder_type;
 
     builder_trace (b : builder_type) :
-      ChainTrace empty_env [] (builder_env b) [];
+      inhabited (ChainTrace empty_env [] (builder_env b) []);
   }.
 
 Global Coercion builder_type : ChainBuilderType >-> Sortclass.
